reorganize into src/Disks/ and src/Refinements/

src/Disks/ZonedDisk.dfy
@@ -1,50 +1,59 @@
-include "Types.dfy"
+include "./BlockDisk.dfy"
+include "../Types.dfy"
 
 // A read-anywhere, append-only datatype.
 module Zone {
     import opened NativeTypes
+    import Block
 
-    datatype Constants = Constants(
-        block_sz: usize
-    )
-
-    class Variables {
+    const block_sz := 1024;
+    
+    class State
+    {
         var write_ptr: usize
-        var bytes: seq<uint8>
+        var blocks: seq<Block.State>
 
         function Valid() : bool 
-            reads this;
+            reads this
         {
-            0 < |bytes| < 0x1_0000_0000_0000_0000
-            && 0 <= write_ptr as int < |bytes|
+            0 < |blocks| < USIZE_MAX
+            && 0 <= write_ptr as int < |blocks|
         }
 
-        constructor Init(sz: usize)
-            requires sz > 0
+        constructor New(blocks: usize)
+            // XXX: email Robin about why we have to bound USIZE_MAX given the argument to Init
+            requires 0 < blocks as int < USIZE_MAX
             ensures Valid()
         {
             this.write_ptr := 0;
-            this.bytes := seq(sz, i => 0);
+            this.blocks := seq(blocks, i => Block.Init());
         }
 
-        function method Read(offset: int, len: int) : seq<uint8>
+        function method Read(offset: usize) : Block.State
             reads this
-            requires offset >= 0
-            requires len > 0
-            requires offset + len < |bytes|
+            requires Valid()
+            requires 0 <= offset < write_ptr
         {
-            bytes[offset .. offset + len]
+            blocks[offset]
         }
 
-        method Write(data: seq<uint8>)
+        method Write(data: Block.State)
             modifies this
             requires Valid()
-            requires write_ptr as int + |data| < |bytes|
-            ensures old(|bytes|) == |bytes|
+            requires |data| % block_sz == 0
+            requires write_ptr as int < |blocks| - 1
             ensures Valid()
         {
-            bytes := bytes[..write_ptr] + data + bytes[(write_ptr as int + |data|)..];
-            write_ptr := write_ptr + |data| as usize;
+            blocks := blocks[write_ptr := data];
+            write_ptr := write_ptr + 1;
+        }
+
+        method Reset()
+            modifies this
+            requires Valid()
+            ensures Valid()
+        {
+            write_ptr := 0;
         }
     }
 }
@@ -52,18 +61,26 @@ module Zone {
 module ZonedDisk /* refines TrackedDisk */ {
     import opened NativeTypes
     import opened Types
+    import opened Zone
 
     datatype Constants = Constants(
-        drive_sz: uint64,
+        n_blocks: uint64,
         zone_map: seq<(uint64, uint64)> // [b, e)
     )
 
-    predicate zone_map_well_formed(drive_sz: uint64, zone_map: seq<(uint64, uint64)>)
+    // TODO: for crash consistency, we ought to distinguish between persistent state
+    // and in-memory state (and show, presuamably, that at all steps the latter can be
+    // reconstructed from the former?)
+    datatype State = State(
+        zones: seq<Zone.State>
+    )
+
+    predicate zone_map_well_formed(n_blocks: uint64, zone_map: seq<(uint64, uint64)>)
     {
-        drive_sz > 0
-        && 0 < |zone_map| < drive_sz as int
+        n_blocks > 0
+        && 0 < |zone_map| as int
         && zone_map[0].0 == 0
-        && zone_map[|zone_map| - 1].1 == drive_sz
+        && zone_map[|zone_map| - 1].1 == n_blocks
         && forall i :: 0 <= i < |zone_map| ==> zone_map[i].0 < zone_map[i].1
         && forall i :: 0 <= i < |zone_map| - 1 ==> zone_map[i].1 == zone_map[i+1].0
         // TODO: email Robin about triggering with the following uncommented...
@@ -72,11 +89,11 @@ module ZonedDisk /* refines TrackedDisk */ {
     }
 
     method resolve_lba(c: Constants, lba: uint64) returns (zone: int, offset: uint64) 
-        requires 0 <= lba < c.drive_sz
-        requires zone_map_well_formed(c.drive_sz, c.zone_map)
+        requires 0 <= lba < c.n_blocks
+        requires zone_map_well_formed(c.n_blocks, c.zone_map)
 
         ensures 0 <= zone < |c.zone_map|
-        ensures 0 <= c.zone_map[zone].0 < c.drive_sz
+        ensures 0 <= c.zone_map[zone].0 < c.n_blocks
         ensures 0 <= offset < c.zone_map[zone].1
         ensures c.zone_map[zone].0 <= lba;
         ensures offset == lba - c.zone_map[zone].0;
@@ -96,7 +113,13 @@ module ZonedDisk /* refines TrackedDisk */ {
         }
     }
 
-    datatype State = State(validTracks: set<uint32>)
+    predicate Valid(c: Constants, s: State) 
+        requires zone_map_well_formed(c.n_blocks, c.zone_map)
+        reads s.zones
+    {
+        |s.zones| == |c.zone_map|
+    }
+
     datatype Step =
     | ReadBlock(block: uint32, contents: seq<uint8>)
     | WriteBlock(tid: uint32, contents: seq<uint8>)
