src/Types.dfy
@@ -1,8 +1,14 @@
 module NativeTypes {
-    newtype{:nativeType "byte" } uint8 = i:int | 0 <= i < 0x100
-    newtype{:nativeType "ulong"} uint32 = i:int | 0 <= i < 0x1_0000_0000
-    newtype{:nativeType "ulong"} uint64 = i:int | 0 <= i < 0x1_0000_0000_0000_0000
-    newtype{:nativeType "ulong"} usize  = i:int | 0 <= i < 0x1_0000_0000_0000_0000
+    const UINT8_MAX := 0x100 - 1
+    const UINT32_MAX := 0x1_0000_0000 - 1
+    const UINT64_MAX := 0x1_0000_0000_0000_0000 - 1
+    const USIZE_MAX := UINT64_MAX
+
+    newtype{:nativeType "byte" } uint8 = i:int | 0 <= i <= UINT8_MAX
+    newtype{:nativeType "ulong"} uint32 = i:int | 0 <= i <= UINT32_MAX
+    newtype{:nativeType "ulong"} uint64 = i:int | 0 <= i <= UINT64_MAX
+    newtype{:nativeType "ulong"} usize  = i:int | 0 <= i <= USIZE_MAX
+
 }
 
 module Types {
