src/Disks/BlockDisk.dfy
@@ -1,0 +1,121 @@
+include "../Types.dfy"
+
+module Block {
+    import opened NativeTypes
+
+    // XXX: Can I parameterise this "module parameter"?
+    const block_sz := 1024;
+
+    type State = seq<uint8>
+
+    predicate Valid(s: State) {
+        |s| == block_sz
+    }
+
+    function method Init() : State
+        ensures Valid(Init())
+    {
+        seq(block_sz, i => 0)
+    }
+}
+
+module BlockDisk {
+    import opened NativeTypes
+    import opened Types
+    import opened Block
+
+    datatype Constants = Constants(
+        n_blocks: uint32
+    )
+    datatype State = State(
+        // XXX: should this be seq<option<Block>> ?
+        blocks: seq<Block.State>
+    )
+
+    predicate ConstantsValid(c: Constants) {
+        && c.n_blocks > 0
+    }
+
+    predicate Valid(c: Constants, s: State) 
+    {
+        && ConstantsValid(c)
+        && |s.blocks| == c.n_blocks as int
+        && forall i :: 0 <= i < |s.blocks| ==> Block.Valid(s.blocks[i])
+    }
+
+    function method Init(c: Constants) : State 
+        requires ConstantsValid(c)
+        ensures Valid(c, Init(c))
+    {
+        State(seq(c.n_blocks, i => Block.Init()))
+    }
+
+    function method Read(c: Constants, s: State, block_id: int) : Block.State
+        requires Valid(c, s)
+        requires 0 <= block_id < |s.blocks|
+        ensures Block.Valid(Read(c, s, block_id))
+    {
+        s.blocks[block_id]
+    }
+
+    predicate Write(c: Constants, s: State, s': State, block_id: int, val: Block.State)
+        requires Valid(c, s)
+    {
+        && 0 <= block_id < |s.blocks|
+        && Block.Valid(val)
+        && s'.blocks == s.blocks[block_id := val]
+    }
+
+    // Invariant preservation
+
+    lemma InitImpliesValid(c: Constants, s: State) 
+        requires ConstantsValid(c)
+        requires s == Init(c)
+        ensures Valid(c, s)
+    {}
+
+    lemma ReadPreservesValid(c: Constants, s: State, s': State, block_id: int, val: Block.State)
+        requires Valid(c, s)
+        requires s == s'
+        requires 0 <= block_id as int < |s.blocks|
+        requires Read(c, s, block_id) == val
+        ensures Valid(c, s')
+    {
+    }
+    
+    lemma WritePreservesValid(c: Constants, s: State, s': State, block_id: int, val: Block.State)
+        requires Valid(c, s)
+        requires 0 <= block_id as int < |s.blocks|
+        requires Write(c, s, s', block_id, val)
+        ensures Valid(c, s')
+    {
+    }
+
+    // Step relations
+
+    datatype Step =
+    | ReadBlock(id: int, val: Block.State)
+    | WriteBlock(b: int, val: Block.State)
+
+    predicate ValidStep(c: Constants, s: State, s': State, step: Step)
+    {
+        match step {
+            case ReadBlock(off, val) => && 0 <= off as int < |s.blocks| 
+                                      && Valid(c, s)
+                                      && Valid(c, s')
+                                      && s == s'
+                                      && s.blocks[off] == val
+            case WriteBlock(off, val) => && 0 <= off as int < |s.blocks|
+                                       && Valid(c, s)
+                                       && Valid(c, s')
+                                       && Block.Valid(val)
+                                       && s'.blocks == s.blocks[off := val]
+        }       
+    }
+
+    predicate Next(c: Constants, s: State, s': State)
+    {
+        exists step :: ValidStep(c, s, s', step)
+    }
+
+}
