src/Refinements/BlockDiskRefinesItself.dfy
@@ -1,0 +1,52 @@
+include "../Types.dfy"
+include "../Disks/BlockDisk.dfy"
+
+import opened NativeTypes
+
+import C = BlockDisk
+import A = BlockDisk
+import opened Block
+
+function IC(c: C.Constants): A.Constants
+{
+    c
+}
+
+function I(c: C.Constants, s: C.State): A.State
+    requires C.ConstantsValid(c)
+    requires C.Valid(c,s)
+    ensures A.Valid(IC(c), I(c, s))
+{
+    s
+}
+
+lemma RefinesInit(c: C.Constants)
+    requires C.ConstantsValid(c)
+    requires C.Valid(c, C.Init(c))
+    ensures A.Valid(IC(c), I(c, C.Init(c)))
+{}
+
+lemma RefinesReadStep(c: C.Constants, s: C.State, s': C.State, block_id: int, val: Block.State)
+    requires C.ValidStep(c, s, s', C.ReadBlock(block_id, val))
+    requires C.Read(c, s, block_id) == val
+    ensures A.Read(IC(c), I(c, s), block_id) == val
+{
+}
+
+lemma RefinesWriteStep(c: C.Constants, s: C.State, s': C.State, block_id: int, val: Block.State)
+    requires C.ValidStep(c, s, s', C.WriteBlock(block_id, val))
+    requires C.Write(c, s, s', block_id, val)
+    ensures A.Write(IC(c), I(c, s), I(c, s'), block_id, val)
+{
+}
+
+lemma RefinesStep(c: C.Constants, s: C.State, s': C.State, step: C.Step)
+    requires C.ConstantsValid(c)
+    requires C.ValidStep(c, s, s', step)
+    ensures A.Next(IC(c), I(c, s), I(c, s'))
+{
+    match step {
+        case ReadBlock(b, val) => RefinesReadStep(c, s, s', b, val);
+        case WriteBlock(b, val) => RefinesWriteStep(c, s, s', b, val);
+    }
+}
